Suma_particion

CODIGO/SUMA/Transformations/SumaToIntervalo.dfy
@@ -1,42 +1,42 @@
 include "../Auxiliar/Sum.dfy"
-include "../Problems/Suma.dfy"
+include "../Problems/SumaNat.dfy"
 include "../Problems/Intervalo.dfy"
 
 
-function Suma_To_Intervalo(A:multiset<int>, S:int) : (r:(multiset<int>, int, int))
+function Suma_to_Intervalo(A:multiset<nat>, S:nat) : (r:(multiset<nat>, nat, nat))
 {
     (A, S, S+1)
 }
 
-lemma Suma_Intervalo(A:multiset<int>, S:int)
-  ensures var (IE,IS,IT) := Suma_To_Intervalo(A, S);
+lemma Suma_Intervalo(A:multiset<nat>, S:nat)
+  ensures var (IE,IS,IT) := Suma_to_Intervalo(A, S);
           Suma(A,S) <==> Intervalo(IE,IS,IT)
 { 
     Suma_Intervalo1(A,S);
     Suma_Intervalo2(A,S);
 }
 
-lemma Suma_Intervalo1(A:multiset<int>, S:int)
-    ensures var (IE,IS,IT) := Suma_To_Intervalo(A, S);
+lemma Suma_Intervalo1(A:multiset<nat>, S:nat)
+    ensures var (IE,IS,IT) := Suma_to_Intervalo(A, S);
           Suma(A,S) <== Intervalo(IE,IS,IT)
 {   
-    var (IE,IS,IT) := Suma_To_Intervalo(A,S);
+    var (IE,IS,IT) := Suma_to_Intervalo(A,S);
     // IE = {1, 2, 4}, IS = 6, IT = 7
     if (Intervalo(IE,IS,IT)) {
-        var C:multiset<int> :| C <= A && IS <= GSumInt(C) < IT; // C = 2, 4  ->  Sum(C) = 6
-        assert GSumInt(C) == S; // Sum(C) == 6
+        var C:multiset<int> :| C <= A && IS <= GSumNat(C) < IT; // C = 2, 4  ->  Sum(C) = 6
+        assert GSumNat(C) == S; // Sum(C) == 6
     }
 }
 
-lemma Suma_Intervalo2(A:multiset<int>, S:int)
-    ensures var (IE,IS,IT) := Suma_To_Intervalo(A,S);
+lemma Suma_Intervalo2(A:multiset<nat>, S:nat)
+    ensures var (IE,IS,IT) := Suma_to_Intervalo(A,S);
           Suma(A,S) ==> Intervalo(IE,IS,IT)
 {
     // A = {1, 2, 4}, S = 6
     if (Suma(A,S)) {
-        var (IE,IS,IT) := Suma_To_Intervalo(A,S);
+        var (IE,IS,IT) := Suma_to_Intervalo(A,S);
 
-        var C:multiset<int> :| C <= A && GSumInt(C) == S; // C = 2, 4  ->  Sum(C) = 6
-        assert IS <= GSumInt(C) < IT; // IS <= 6 < IT
+        var C:multiset<int> :| C <= A && GSumNat(C) == S; // C = 2, 4  ->  Sum(C) = 6
+        assert IS <= GSumNat(C) < IT; // IS <= 6 < IT
     }
 }
