CODIGO/SUMA/Problems/ParticionInt.dfy
@@ -7,5 +7,5 @@ include "../Auxiliar/Sum.dfy"
 ghost predicate Particion(A:multiset<int>)
 {
   exists P1:multiset<int>, P2:multiset<int> | 
-    P1 <= A && P2 <= A && P1 + P2 == A:: GSumInt(P1) == GSumInt(P2)
+    P1 <= A && P2 <= A && P1 + P2 == A :: GSumInt(P1) == GSumInt(P2)
 }
