CODIGO/SUMA/Transformations/SumaToParticion.dfy
@@ -1,6 +1,6 @@
 include "../Auxiliar/Sum.dfy"
-include "../Problems/Suma.dfy"
-include "../Problems/Particion.dfy"
+include "../Problems/SumaInt.dfy"
+include "../Problems/ParticionInt.dfy"
 
 
 function Suma_to_Particion(A:multiset<int>, S:int) : (r:(multiset<int>))
@@ -10,7 +10,7 @@ function Suma_to_Particion(A:multiset<int>, S:int) : (r:(multiset<int>))
 }
 
 lemma Suma_Particion(A:multiset<int>, S:int)
-  ensures var (PA) := Suma_to_Particion(A, S);
+  ensures var PA := Suma_to_Particion(A, S);
           Suma(A,S) <==> Particion(PA)
 { 
     Suma_Particion1(A,S);
@@ -18,26 +18,43 @@ lemma Suma_Particion(A:multiset<int>, S:int)
 }
 
 lemma Suma_Particion1(A:multiset<int>, S:int)
-    ensures var (PA) := Suma_to_Particion(A, S);
+    ensures var PA := Suma_to_Particion(A, S);
           Suma(A,S) <== Particion(PA)
 {   
-    var (PA) := Suma_To_Intervalo(A,S);
-    // PA = {1, 2, 3, 4, 2(N)}
+    var PA := Suma_to_Particion(A,S);
+    // PA = {1, 2, 3, 4, 2(N)}   
+    // S = 6
     if (Particion(PA)) {
-        var C:multiset<int> :| C <= A && IS <= GSum(C) < IT; // C = 2, 4  ->  Sum(C) = 6
-        assert GSum(C) == S; // Sum(C) == 6
+        var N := 2*S - FSumInt(A); // N = 2
+        var PA' := PA - multiset{N}; // PA' = {1, 2, 3, 4} 
+        
+        var P1 :multiset<int> :| P1 <= PA' && GSumInt(P1) == S; // P1 = {2, 4}  ->  Sum(P1) = 6
+        var P2 := PA' - P1 + multiset{N}; // P2 = {1, 3, 2} -> Sum(P2) = 6
+
+        assert PA' <= PA && GSumInt(P1) == S; // Sum(C) == 6
     }
 }
 
 lemma Suma_Particion2(A:multiset<int>, S:int)
-    ensures var (PA) := Suma_to_Particion(A, S);
+    ensures var PA := Suma_to_Particion(A, S);
           Suma(A,S) ==> Particion(PA)
 {
-    // A = {1, 2, 4}, S = 6
+    // A = {1, 2, 3, 4}, S = 6
     if (Suma(A,S)) {
-        var (PA) := Suma_To_Intervalo(A,S);
+        var N := 2*S - FSumInt(A); // N = 2
+        var PA := Suma_to_Particion(A,S);
 
-        var C:multiset<int> :| C <= A && GSum(C) == S; // C = 2, 4  ->  Sum(C) = 6
-        assert IS <= GSum(C) < IT; // IS <= 6 < IT
+        var P1 : multiset<int> :| P1 <= A && GSumInt(P1) == S; // P1 = {2, 4}  ->  Sum(P1) = 6
+        var R := A - P1; // R = {1, 3}
+        var P2 := R + multiset{N}; // P2 = {1, 3, 2} -> Sum(P2) = 6
+        
+        assert GSumInt(P1) == S;
+        assert GSumInt(P2) == S;
+
+        assert A == P1 + R;
+        assert GSumInt(A) == GSumInt(P1) + GSumInt(R);
+        assert N == 2*S - GSumInt(A) == S - GSumInt(R);
+
+        assert GSumInt(P1) == GSumInt(P2) == S && P1 + P2 == PA ; // N in PA && GSumInt(C) == GSumInt(PA') == S && C + PA' == PA; // IS <= 6 < IT
     }
 }
